\documentclass[class=article, crop=false]{standalone}
\usepackage[utf8]{inputenc}

\newcommand{\xdownarrow}[1]{%
  {\left\downarrow\vbox to #1{}\right.\kern-\nulldelimiterspace}
}
\usepackage{latexsym}
  \usepackage{comment}
  \usepackage{showlabels}
  \usepackage{amsmath,amsthm,amsfonts,amssymb,graphicx,epsfig,latexsym,color,amssymb}
  %\usepackage{showkeys}
  \usepackage{epsf}
  \usepackage{enumitem}
  \usepackage{tikz}
  \usepackage{tikz-cd}
  \def\rank{\operatorname{rank}}

\newcommand{\bbfamily}{\fontencoding{U}\fontfamily{bbold}\selectfont}
\DeclareMathAlphabet{\mathbbold}{U}{bbold}{m}{n}
\begin{document}
\begin{center}
    Proof of Local Tate Duality
\end{center}
Fix $K/\mathbb{Q}_p$ a finite extension. Let $M$ be a $G_K$-module. 
\vskip 5pt
\textbf{Definition}: We let $M^* = \text{Hom}(M, \mu_{\infty})$ denote the \textit{Tate Dual} of $M$. 
\vskip 5pt 
Let $\phi \in M^*$, $g\in G_K$. We define $(g\phi)(m)=g\phi(g^{-1}m)$. 
\vskip 5pt 
\textbf{Example}: $M=\mathbb{Z}/n$ with trivial $G_K$ action gives $M^*\cong \mu_{n}\subset \overline{K}$. Essentially the Tate Dual in this case equips $\mathbb{Z}/n$ with some natural $G_K$ action.
\vskip 5pt
We obtain a $G_K$ equivariant pairing
\[M\times M^* \to \mu_{\infty}\]
\[(m, \phi) \mapsto \phi(m)\]
This induces the \textit{duality map}

\begin{tikzcd}
{\langle \cdot, \cdot \rangle_K:H^i(G_K,M)\times H^{2-i}(G_K,M^*)} \arrow[r, "\cup"] \arrow[rrd, "{\langle \cdot, \cdot \rangle_K}"'] & {H^2(G_K, M \otimes_{\mathbb{Z}}M^*)} \arrow[r] & {H^2(G_K,\mu_{\infty})} \arrow[d, "inv_K", "\sim"'] \\
                                                                                                                                      &                                                 & \mathbb{Q}/\mathbb{Z}      
\end{tikzcd}

\textbf{Theorem}: Suppose $|M|<\infty$. $\langle \cdot, \cdot \rangle_K$ is a perfect pairing for $i=0,1,2$. 
\vskip 3pt That is, it induces isomorphisms \[H^i(G_K,M) \to H^{2-i}(G_K, M^{*})^{\vee}, \quad  H^{2-i}(G_K,M^{*}) \to H^i(G_K, M)^{\vee},\]
with $D^{\vee} = \text{Hom}(D, \mathbb{Q}/\mathbb{Z})$, homomorphisms in Ab.
\vskip 5pt
The proof will be in two parts, when $i=2$ and when $i=1$. $i=0$ follows from $i=2$ and the symmetry of the pairing (just dualize the isomorphisms). The $i=1$ will utilize the $i=2$ case and dimension shifting, so we prove $i=2$ first.

\begin{proof}
$(i=2)$. We have $H^0(K,M^*)=(M^*)^{G_K}=\text{Hom}_{G_K}(M, \mu_{\infty})$, for if $\phi \in (M^*)^{G_K}$, then $\phi(gm)=(g\phi)(gm)=g\phi(g^{-1}gm)=g\phi(m)$. The other direction is similar.
\par 
$\phi \in \text{Hom}_{G_K}(M,\mu_{\infty})$ induces a map $H^2(G_K,M) \to H^2(G_K,\mu_{\infty})$ by evaluation, which we also denote by $\phi$. The duality map then identifies to
\[\Theta_K:\text{Hom}_{G_K}(M, \mu_{\infty}) \to H^2(G_K,M)^{\vee}\]
\[\phi \mapsto \text{inv}_K\circ \phi :H^2(G_K,M)\to \mathbb{Q}/\mathbb{Z}\]
Our goal is to show $\Theta_K$ is an isomorphism. To do this, we will use a similar trick to JJ's spectral sequence argument. We will take a cleverly chosen finite extension $L/K$ so that $L$ is "simple". First we want to know that understanding the corresponding $\Theta_L$ maps gives us information about $\Theta_K$. This is contained in the following two claims:
\vskip 5pt
\textbf{Claim 1}: The following diagram commutes.
\[\begin{tikzcd}
{Hom_{G_K}(M,\mu_{\infty})} \arrow[r, "\Theta_K"] \arrow[d, hook] & {H^2(G_K, M)^{\vee}} \arrow[d, "cor^{\vee}", dashed] \\
{Hom_{G_L}(M,\mu_{\infty})} \arrow[r, "\Theta_L"]                 & {H^2(G_L,M)^{\vee}}                                 
\end{tikzcd}\]
\textit{Proof of claim}: We have the following commutative diagram
\[\begin{tikzcd}
{H^2(G_L,M) } \arrow[rrd, "\varphi"] \arrow[r, "cor"] & {H^2(G_K,M)} \arrow[r, "\varphi"] & {H^2(G_K,\mu_{\infty})} \arrow[r, "Inv_K"]                    & \mathbb{Q}/\mathbb{Z}                             \\
                                                      &                                   & {H^2(G_L,\mu_{\infty})} \arrow[r, "Inv_L"] \arrow[u, "cor"] & \mathbb{Q}/\mathbb{Z} \arrow[u, "Id", Rightarrow]
\end{tikzcd}\]
The triangle on the left commutes because cor commutes with maps of Galois modules. The square on the right commutes by the final result of Sriram's talk.
\par 
\mbox{}\hfill \qedsymbol
\\
\textbf{Claim 2}: $\text{cor}^{\vee}$ is injective, and thus [$\Theta_L$ an isomorphism implies $\Theta_K$ an isomorphism]
\\
\textit{Proof of claim}: Let us first assume cor$^{\vee}$ is injective. Suppose $\Theta_L$ is an isomorphism. Since $\Theta_L$ is $G(L/K)$ equivariant (Seen by direct calculation by writing $G(L/K)=G_K/G_L$),
\[\begin{tikzcd}
{Hom_{G_K}(M,\mu_{\infty})=Hom_{G_L}(M,\mu_{\infty})^{G(L/K)}} \arrow[rd, "\Theta_K"'] \arrow[r, "\Theta_L"] & {(H^2(G_L,M)^{\vee}))^{G(L/K)}}                      \\
                                                                                                                & {H^2(G_K,M)^{\vee}} \arrow[u, "cor^{\vee}"', hook]
\end{tikzcd}\]
is a commutative diagram by claim $1$. Thus since $\Theta_L$ is an isomorphism, so is $\Theta_K$.
\vskip 3pt
To show that cor$^{\vee}$ is injective, we show cor is surjective. Recall that cor is constructed so that, if $\Phi:H^2(G_K, \text{Ind}_{G_L}^{G_K}M) \to H^2(G_L,M)$ is the isomorphism given by Shapiro's lemma, then $tr:\text{Ind}_{G_L}^{G_K}M \to M = \text{cor}\circ \Phi$, with $tr(\phi) = \sum_{g\in G_K/G_L}g^{-1}\phi(g)$. One easily sees that tr is surjective, so since $H^3(G_K, \text{ker}(tr)) = 0$, the long exact sequence induced by tr implies that cor is surjective.
\par 
\mbox{}\hfill \qedsymbol
\\
Following the technique illustrated by JJ's talk, we choose $L/K$ finite so that $G_L$ acts on both $M$ and $\mu_{|M|}$ trivially. Thus $M$ as a $G_L$ module is a sum of $\mu_{n_i}$'s, so for our purposes we may assume $M=\mu_n$ for some $n$.
\vskip 5pt
The proof then follows by noting the obvious commutativity of the following diagram.
\[\begin{tikzcd}
(x\mapsto x^r)       & {Hom_{G_K}(\mu_n, \mu_{\infty})} \arrow[r, "\Theta_L"] & {H^2(G_K, \mu_n)^{\vee}}                                                                   \\
r \arrow[u, maps to] & \mathbb{Z}/n \arrow[u, "\sim"] \arrow[r, "\sim"]       & {Hom((\frac{1}{n}\mathbb{Z})/\mathbb{Z}, \mathbb{Q}/\mathbb{Z})} \arrow[u, "inv_K^{\vee}"] \\
                     & r \arrow[r, maps to]                                   & (\frac{1}{n} \mapsto \frac{r}{n})                                                         
\end{tikzcd}\]
$(i=1)$: We want to apply dimension shifting. The problem is, in dimension shifting we have to deal with a $G_K$ module which is not finite, so we won't be able to apply our $i=2/i=0$ cases.
\vskip 5pt
But the cohomology of $G_K$ with coefficients in Ind$_1^{G_K}M$ can naturally be written as the direct limit of the cohomology of $G_K$ with coefficients in finite submodules of Ind$_1^{G_K}M$. Thus $M$ must embed in some finite submodule $N$ of Ind$_1^{G_K}M$ such that $H^j(G_K,N)=0$ for $j\geq 1$.
\vskip 5pt 
Then we have the SES's
\[0 \to M \to N \to Q \to 0\]
\[0 \to Q^* \to N^* \to M^* \to 0\]
And these show that
\[H^0(G_K, N) \to H^0(G_K, Q) \to H^1(G_K, M) \to 0\]
\[H^2(G_K,N^*)^{\vee} \to H^2(G_K,Q^*)^{\vee} \to H^1(G_K,M^*)^{\vee}\]
are exact. 
\vskip 5pt
These give rise to the commutative diagram
\[\begin{tikzcd}
{H^0(G_K,N)} \arrow[r] \arrow[d, "\sim"'] & {H^0(G_K, Q)} \arrow[r] \arrow[d, "\sim"'] & {H^1(G_K,M)} \arrow[r] \arrow[d] & 0 \\
{H^2(K, N^*)^{\vee}} \arrow[r]            & {H^2(G_K, Q^*)^{\vee}} \arrow[r]           & {H^1(G_K,M^*)^{\vee}}            &  
\end{tikzcd}\]
with exact rows. The left hand vertical arrows are isomorphisms by the $i=2/i=0$ cases of the theorem. 
\vskip 5pt
By a diagram chase, $H^1(G_K,M) \hookrightarrow H^1(G_K, M^*)^{\vee}$, and by symmetry $H^1(G_K, M^*) \hookrightarrow H^1(G_K, M)^{\vee}$ so 
\begin{tikzcd} 
H^1(G_K,M) \arrow[r, tail, twoheadrightarrow] & H^1(G_K,M^*)^{\vee}
\end{tikzcd}
Thus the finite groups have the same order, so the maps must be isomorphisms.
\end{proof}

Let us now establish a few functorial properties of the pairing.
\vskip 5pt 
\textbf{Theorem}: The duality map $\langle \cdot, \cdot \rangle_K: H^i(G_K,M)\times H^{2-i}(G_K,M^*) \to \mathbb{Q}/\mathbb{Z}$ satisfies the following properties:
\begin{enumerate}
    \item Given $L/K$ finite, $x\in H^i(G_K,M)$, $y\in H^{2-i}(G_L, M^*)$, we have $\langle x, \text{cor}(y)\rangle_K = \langle \text{res}(x), y\rangle_L$.
    \item With the same notation as above, $\langle \text{res}(x), \text{res}(y)\rangle_L = [L:K]\langle x, y \rangle_K$.
\end{enumerate}
\begin{proof}
\begin{enumerate}
    \item We have \[\langle x, \text{cor}(y)\rangle_K = inv_K(x \cup \text{cor}(y)) = inv_K(\text{cor}(\text{res}(x)\cup y)) = inv_L(\text{res}(x)\cup y) = \langle \text{res}(x),y\rangle_L.\]
    \item We have \[\langle \text{res}(x), \text{res}(y)\rangle= inv_L(\text{res}(x)\cup \text{res}(y)) = inv_L(\text{res}(x\cup y)) = [L:K]\langle x, y \rangle_K.\]
\end{enumerate}
The proofs for $\text{res}(x)\cup \text{res}(y) = \text{res}(x\cup y)$ and $x \cup \text{cor}(y) = \text{cor}(\text{res}(x)\cup y)$ are partially illustrated in "ATIYAH, M. F. AND WALL, C. T. C. 1967. Cohomology of groups, pp. 94â€“115. In Algebraic Number Theory (Proc. Instructional Conf., Brighton, 1965). Thompson, Washington, D.C." (Which I found on google scholar).
\end{proof}
\end{document}
